Defined strict initial and strict terminal objects and proved the appropriate instances.

Universal/Initial.v
@@ -135,3 +135,12 @@ Proof.
 Qed.
 
 End wut.
+
+Class HasStrictInit (C : Cat) {hi : HasInit C} : Prop :=
+  isStrictlyInitial : forall {X : Ob C} (f : Hom X (init C)), isIso f.
+
+#[export] Hint Mode HasStrictInit ! ! : core.
+#[export] Hint Mode HasStrictInit ! - : core.
+
+Arguments HasStrictInit _ {hi}.
+Arguments isStrictlyInitial {C hi _} _.
